<?xml version="1.0" encoding="utf-8"?>
<section xmlns:xi="http://www.w3.org/2001/XInclude">
  <title></title>
  <subsection>
    <title>Motivation</title>
    <p>
      Differential equations are prevalent because the world is dynamical. The dimension of time is very different from the three spatial dimensions. The universe is not frozen at <url href="https://en.wikipedia.org/wiki/Absolute_zero">absolute zero</url>, nor is it in the <url href="https://en.wikipedia.org/wiki/Heat_death_of_the_universe">heat death</url>. Things move around.
    </p>
    <p>
      This is the prime example of differential equations: speed implies movement. Say at time <m>t</m> something is at position <m> x (t) </m>. Prescribing the speed as a function of time sets up a differential equation. Say  <m> x' (t) = 100 </m>. The <em>general</em> solution can be found by
      <md>
        <mrow> \sd x \amp= 100 \sd t\text{,} \amp \int \sd x \amp= \int 100 \sd t\text{,} \amp x \amp= 100 t + C\text{.} </mrow>
      </md>
      This is a family of solutions parameterized by a parameter <m>C</m>. Think of <m>C</m> as a radio knob or a slider bar: tweaking it gives different functions <m> x (t) </m>. An extra condition pins down the parameter and thus gives a <em>specific</em> solution. Say <m> x (1) = 0 </m>. Then <m> C = -100 </m> and <m> x (t) = -100 + 100 t </m>. 
    </p>
    <p>
      An equivalent way to write the solution is through
      <me>
        x (t) = x (0) + \int_0^t x' (s) \sd s = x (0) + 100 t
      </me>.
      This is very physical because
      <ol>
        <li>
          <p>
            we are able to start from any starting point <m> x (0) </m> (solution exists for any initial value), and
          </p>
        </li>
        <li>
          <p>
            the starting point <m> x (0) </m> completely determines the trajectory <m> x (t) </m> (the solution is unique for any initial value).
          </p>
        </li>
      </ol>
    </p>
    <p>
      The more physical example involves forces:
      <md>
        <mrow> \ddot{x} \amp= \frac{1}{m} F\text{,} \amp \text{or equivalently} \quad \amp\left\{\begin{aligned} \dot{x} \amp= \frac{1}{m} p \text{,} \\ \dot{p} \amp= F\text{.} \end{aligned}\right. </mrow>
      </md>
      This, classical mechanics, is all of physics, before
      <ul>
        <li>
          <p>
            continuum/field theory (too many small discrete things together form a <url href="https://en.wikipedia.org/wiki/Continuum_mechanics">continuous entity</url>),
          </p>
        </li>
        <li>
          <p>
            statistical mechanics (the initial condition is <url href="https://en.wikipedia.org/wiki/Ergodic_hypothesis">too complicated</url> to be described unless statistically), and
          </p>
        </li>
        <li>
          <p>
            quantum mechanics (the trajectory is <url href="https://en.wikipedia.org/wiki/Uncertainty_principle">inherently non-deterministic</url>).
          </p>
        </li>
      </ul>
    </p>
    <assemblage>
      <title>Principle α</title>
      <p>
        A differential equation is always an equation of functions. The general solution is a parameterized family of functions. Extra conditions pin down the parameters and yield specific solutions.
      </p>
    </assemblage>
  </subsection>
  <subsection>
    <title>Linearity</title>
    <p>
      An operation being linear means addition goes through the operation, <ie/>
      <me>
        F ( x + y ) = F (x) + F (y)
      </me>.
      (The operation of) multiplying by <m>2</m> is linear:
      <md>
        <mrow> 2 \times ( 5 + 7 ) \amp= 2 \times 5 + 2 \times 7\text{,} \amp 2 ( a + b ) \amp= 2 a + 2 b\text{.} </mrow>
      </md>
      Taking derivatives is linear:
      <me>
        ( f (x) + g (x) )' = f' (x) + g' (x)
      </me>,
      and multiplying by a function is also linear:
      <me>
        h (x) ( f (x) + g (x) ) = h (x) f (x) + h (x) g (x)
      </me>.
      However, most of the things are not linear, especially like (unless for very special values)
      <md>
        <mrow> ( a + b )^2 \amp\neq a^2 + b^2\text{,} \amp \frac{1}{ a + b } \amp\neq \frac{1}{a} + \frac{1}{b}\text{,} \amp \se^{ a + b } \amp\neq \se^a + \se^b\text{.} </mrow>
      </md>
      Taylor expansion says as long as we look close enough, a (nice) non-linear thing will <em>locally</em> almost look like a linear thing.
      However, most of the interesting yet complicated behaviors are still brought by non-linearity <em>globally</em>.
    </p>
    <p>
      Solutions of (homogenous) linear differential equations can be added because of linearity:
      <md alignment="alignat">
        <mrow> y' (x) \amp- ( \sin x ) \amp y (x) \amp= 0\text{,} </mrow>
        <mrow> z' (x) \amp- ( \sin x ) \amp z (x) \amp= 0\text{,} </mrow>
        <mrow> \text{then} \quad ( y (x) + z (x) )' \amp- ( \sin x ) \amp ( y (x) + z (x) ) \amp= 0\text{,} </mrow>
      </md>
      or more generally for linear combinations:
      <me>
       \quad ( a y (x) + b z (x) )' - ( \sin x ) ( a y (x) + b z (x) ) = 0\text{.}
      </me>
      This is exactly like saying solutions to (homogenous) linear systems form a span:
      <md alignment="alignat">
        <mrow> 2 \amp\times 4 \amp + 5 \amp\times 0 \amp + 8 \amp\times (-1) \amp \amp= 0\text{,} </mrow>
        <mrow> 2 \amp\times 1 \amp + 5 \amp\times (-2) \amp + 8 \amp\times 1 \amp \amp= 0\text{,} </mrow>
        <mrow> \text{then} \quad 2 \amp\times ( 4 a + b ) \amp + 5 \amp\times ( -2 b ) \amp + 8 \amp\times ( -a + b ) \amp \amp= 0\text{.} </mrow>
      </md>
    </p>
    <p>
      For linear systems, bases of the solution space (null space) can be found by matrix operations (Gaussian elimination). Linear differential equations are more difficult but there are usually theories providing us with a basis. In other words, we are ensured that the solution can be written as a linear combination of certain functions.
    </p>
    <p>
      Say we have the linear equation <m> y'' - 5 y' + 6 y = 0 </m>. Somebody guarantees us that the solution is a linear combination of functions in the form <m> \se^{ a x } </m> for some <m>a</m>. Plugging <m> y = \se^{ a x } </m> into the differential equation gives <m> ( a^2 - 5 a + 6 ) \se^{ a x } = 0 </m>, so two possible solutions (basis elements) are <m> y = \se^{ 2 x } </m> and <m> y = \se^{ 3 x } </m>. The general solution is therefore linear combinations
      <me>
        y = A \se^{ 2 x } + B \se^{ 3 x }
      </me>,
      which has two parameters <m>A</m> and <m>B</m> that can take arbitrary values.
    </p>
    <p>
      If we are given the initial conditions <m> y (0) = 0 </m> and <m> y' (0) = 1 </m>, we want to figure out what exact values of <m>A</m> and <m>B</m> will make these happen. Plugging in again, we see <m> y (0) = A + B = 0 </m> and <m> y' (0) = 2 A + 3 B = 1 </m>. So <m> A = -1 </m> and <m> B = 1 </m>, <ie/> the specific solution is <m> y (x) = -\se^{ 2 x } + \se^{ 3 x } </m>.
    </p>
    <assemblage>
      <title>Principle β</title>
      <p>
        For linear differential equations, past hard work of physicists and mathematicians (which? vote!) gives us some functions such that (1) any linear combination of them is a solution and (2) any solution is a linear combination of them. The general solution is any linear combination, and the specific solution is some linear combination.
      </p>
    </assemblage>
  </subsection>
  <subsection>
    <title>Jacobian</title>
    <p>
      A function <m> y (x) </m> tells how a variable <m>y</m> associates with another variable <m>x</m>. Say <m> y (x) = \se^x </m>:
      <tabular halign="center">
        <row bottom="minor">
          <cell><m>x</m></cell>
          <cell><m>y</m></cell>
        </row>
        <row>
          <cell><m>1</m></cell>
          <cell><m>\se</m></cell>
        </row>
        <row>
          <cell><m>2</m></cell>
          <cell><m>\se^2</m></cell>
        </row>
        <row>
          <cell><m>3</m></cell>
          <cell><m>\se^3</m></cell>
        </row>
        <row>
          <cell><m>4</m></cell>
          <cell><m>\se^4</m></cell>
        </row>
      </tabular>
    </p>
    <p>
      If we want to scale the variable <m>y</m> but keep the variable <m>x</m>, we can set up (in variable language)
      <md>
        <mrow> Y \amp= 2 y\text{,} \amp X \amp= x  </mrow>
      </md>,
      <ie/> (in function language)
      <md>
        <mrow> Y (X) = Y (x) = 2 y (x) </mrow>
      </md>.
      In the case of <m> y (x) = \se^x </m>:
      <tabular halign="center">
        <row bottom="minor">
          <cell><m> X = x </m></cell>
          <cell><m>y</m></cell>
          <cell><m>Y</m></cell>
        </row>
        <row>
          <cell><m>1</m></cell>
          <cell><m>\se</m></cell>
          <cell><m> 2 \se </m></cell>
        </row>
        <row>
          <cell><m>2</m></cell>
          <cell><m>\se^2</m></cell>
          <cell><m> 2 \se^2 </m></cell>
        </row>
        <row>
          <cell><m>3</m></cell>
          <cell><m>\se^3</m></cell>
          <cell><m> 2 \se^3 </m></cell>
        </row>
        <row>
          <cell><m>4</m></cell>
          <cell><m>\se^4</m></cell>
          <cell><m> 2 \se^4 </m></cell>
        </row>
      </tabular>
    </p>
    <p>
      The derivative goes intuitively like
      <md>
        <mrow> \frac{ \sd Y }{ \sd X } \amp= \frac{ \sd Y }{ \sd x } = 2 \frac{ \sd y }{ \sd x }\text{,} \amp \sd Y = 2 \sd y </mrow>
      </md>,
      <ie/>
      <me>
        Y' (X) = 2 y' (X) = 2 y' (x)
      </me>.
      This is reasonable because <m>Y</m> changes twice more violently than <m>y</m> with respect to <m> X = x </m>. In the case of <m> y (x) = \se^x </m>, we have <m> Y' (X) = 2 \se^X </m>.
    </p>
    <p>
      If we scale the variable <m>x</m> but keep the variable <m>y</m>, we are relabing the time:
      <md>
        <mrow> Y \amp= y\text{,} \amp X \amp= 2 x\text{.} </mrow>
      </md>
      In the case of <m> y (x) = \se^x </m>:
      <tabular halign="center">
        <row bottom="minor">
          <cell><m>X</m></cell>
          <cell><m>x</m></cell>
          <cell><m> Y = y </m></cell>
        </row>
        <row>
          <cell><m>1</m></cell>
          <cell><m> 1 / 2 </m></cell>
          <cell><m> \se^{ 1 / 2 } </m></cell>
        </row>
        <row>
          <cell><m>2</m></cell>
          <cell><m>1</m></cell>
          <cell><m>\se</m></cell>
        </row>
        <row>
          <cell><m>3</m></cell>
          <cell><m> 3 / 2 </m></cell>
          <cell><m> \se^{ 3 / 2 } </m></cell>
        </row>
        <row>
          <cell><m>4</m></cell>
          <cell><m>2</m></cell>
          <cell><m>\se^2</m></cell>
        </row>
      </tabular>
      Here <m> Y = y </m> changes half slower with respect to <m>X</m> than to <m>x</m>. It's exactly like taking fast-motion pictures in real time of <m>x</m> using a high-speed camera <m> X = 2 x </m>: when playing back in real time of <m>X</m> we are actually seeing slow-motion pictures in half speed <m> x = X / 2 </m>. In function language, all this is saying
      <me>
        Y (X) = y (x) = y \left( \frac{X}{2} \right)
      </me>,
      and the derivative goes counter-intuitively like
      <md>
        <mrow> \frac{ \sd Y }{ \sd X } \amp= \frac{ \sd y }{ \sd X } = \frac{ \sd y }{ \sd x } \frac{ \sd x }{ \sd X } = \frac{1}{2} \frac{ \sd y }{ \sd x }\text{,} \amp \frac{\sd}{ \sd X } \amp= \frac{\sd}{ 2 \sd x } = \frac{1}{2} \frac{\sd}{ \sd x } </mrow>
      </md>,
      <ie/>
      <me>
        Y' (X) = \frac{1}{2} y' \left( \frac{X}{2} \right)
      </me>.
      In the case of <m> y (x) = \se^x </m>, we get <m> Y (X) = \se^{ X / 2 } </m> and <m> Y' (X) = \se^{ X / 2 } / 2 </m>.
    </p>
    <p>
      The two different behaviors have their respective names in field theory or tensor analysis: one called covariant and another contravariant, see <url href="https://en.wikipedia.org/wiki/Covariance_and_contravariance_of_vectors">wiki</url>.
    </p>
  </subsection>
</section>
